crdt_specs2.thy
@@ -1,0 +1,62 @@
+theory crdt_specs2
+  imports crdt_specs
+begin
+
+section "CRDT Specifications Part 2"
+
+text "The previous CRDT are not nice to work with when composed.
+The problem is, that the specifications for maps and structs transform the context
+passed to embedded CRDTs.
+During this transformation the reverse direction is lost, so it is hard to reconstruct the original
+calls from the calls in an embedded context.
+Therefore, we now use a different composition technique, where the mapping is explicitly passed down
+into nested CRDTs."
+
+type_synonym ('op, 'opn, 'res) ccrdtSpec = 
+        "callId set                  \<comment> \<open>visible calls\<close>
+      \<Rightarrow> (callId \<Rightarrow>'op)              \<comment> \<open>call information\<close> 
+      \<Rightarrow> callId rel                  \<comment> \<open>happens-before\<close>
+      \<Rightarrow> ('opn \<Rightarrow> 'op)               \<comment> \<open>mapping back\<close>
+      \<Rightarrow> 'op 
+      \<Rightarrow> 'res
+      \<Rightarrow> bool"
+
+text "There is a mapping between the composable CRDT specs above and the original specifications:"
+
+(* TODO *)
+
+
+subsection "Register"
+
+definition 
+"latest_assignments' vis op hb C \<equiv> 
+   {(c,v). c\<in>vis \<and> op c = C (Assign v) \<and> (\<nexists>c' v'. c'\<in>vis \<and> op c' = C (Assign v') \<and> (c,c')\<in>hb)}"
+
+definition
+"latest_values' vis op hb C \<equiv> snd ` (latest_assignments' vis op hb C)"
+
+definition
+"register_spec' initial vis op hb C oper res \<equiv>
+  case oper of
+    Assign _ \<Rightarrow> res = default
+  | Read \<Rightarrow>
+      if latest_values' vis op hb C = {} then res = initial else res \<in> latest_values' vis op hb C"
+
+
+definition firstValue' :: "'a \<Rightarrow> ('b \<times> 'a) set \<Rightarrow> 'a" where
+"firstValue' d m \<equiv> if m = {} then d else 
+  let maxK = wo_rel.minim some_well_order (fst ` m) in
+  wo_rel.minim some_well_order {y. (maxK,y)\<in>m}
+  "
+
+
+definition 
+"lww_register_spec' initial vis op hb C oper res \<equiv> 
+  case oper of
+    Assign x \<Rightarrow> res = default
+  | Read \<Rightarrow> res = firstValue' initial (latest_values' vis op hb C)"
+
+
+(* Needed for example: structs, set_rw, map_rw *)
+
+end
